\documentclass[11pt]{amsbook}

\usepackage{../HBSuerDemir}


\begin{document}
\hPage{b1p2/289}
and 
\begin{align*}
	&y = x^2  \Rightarrow \ \ \ \sqrt{\frac{1}{2}}  (x' + y') =  \frac{1}{2} (x' - y')^2\\
    \Rightarrow \ \ \ & 
    x'^2 - 2x'y' + y'^2 - 2x' - 2y' = 0
	\intertext{
	\begin{enumerate}
	    \item [3.]	$\tan2\theta = \frac{-3}{1-1} = \infty \Rightarrow 0=\pi/4$,  and  $x^2 - 3xy + y^2 - y = 0$
	\end{enumerate}
	}
	\Rightarrow \ \ \  
    &\frac{1}{2} (x' - y')^2 - \frac{3}{2}(x' - y')(x' + y') + \frac{1}{2}(x' + y')^2 - \frac{1}{2}(x' + y') = 0\\
	\Rightarrow \ \ \ &x'^2 - 2x'y' + y'^2 - 3(x'^2 - y'^2)+(x'^2 + 2x'y' + y'^2)- 2(x' + y') = 0\\
	\Rightarrow \ \ \ &-x'^2 + 5y'^2 - \sqrt{2}x' - \sqrt{2}y' = 0\\
\end{align*}
\begin{exmp}
	Translate the coordinate axes to eliminate the
	linear terms in (1) and compute $\Delta$, $H$, $T$ before and after the
	translation.\\
\begin{align}
	f(x, y) = x^2 + 4xy +2y^2 + x - y -5 = 0
\end{align} 
\end{exmp}
\begin{hSolution}
	Setting  $x = x' + h$, $y = y'+ k$ in (1) we have 
\begin{equation*}
	x'^2 + 4x'y' + 2y'^2 +(2h + 4k + 1)x' + (4h + 4k -1)y' + f(h,k) = 0\\
\end{equation*}
\begin{align*}
	&2h + 4k = -1, \ \ \ \ 4h + 4k = 1 \ \ \ \  h = 1,\ \ \ \ k = -3/4
	\intertext{Then (1) becomes}
	&x'^2 + 4x'y' + 2y'^2 - \frac{33}{8} = 0
\end{align*}
	Now
\begin{align*}
	 &H = A + C = 3,           &&H' = A' + C' = 3\\
	 &\Delta = B^2 - 4AC = 8   &&\Delta' = B'^2 - 4A'C' = 8\\
\end{align*}
	 \indent T =
	$\begin{vmatrix}
		2 & 4 & 1\\
		4 & 4 & -1\\
		1 & -1 & -10
	\end{vmatrix}$
	= 66, \ \ \ \ \ \ \ \ \ \ \ T' = 
	$\begin{vmatrix}
		 2 & 4 & 0\\
		 4 & 4 & 0 \\
		 0 & 0 & \frac{-33}{4}
	\end{vmatrix}$
= 66 
\\
\indent The equalities $H = H'$, $\Delta = \Delta'$ and $T = T'$ observed above are general as proved in the second of the following two theorem 
\end{hSolution}
\end{document}