\documentclass[11pt]{amsbook}

\usepackage[margin=1in,left=1.5in,includefoot]{geometry}
\usepackage{blindtext}
\usepackage{tasks}

\usepackage[utf8]{inputenc}
\usepackage[english]{babel}
 
\newtheorem{theorem}{Theorem}[section]  % to make lema and proof
\newtheorem{corollary}{Corollary}[theorem]
\newtheorem{lemma}[theorem]{Lemma}  

\usepackage{amsfonts}  % make Z and N
\newcommand{\Z}{\mathbb{Z}} 


\begin{document}
% ++++++++++++++++++++++++++++++++++++++
\hpage{fevzioglu-016}
% ++++++++++++++++++++++++++++++++++++++

\begin{proof}We. multiply this relation by $b^{-n}$  on the left and on the right. This gives
$b^{-n}a=ab^{-n}$ for n $\in$ $\mathbb{N}$. So $ab^{n}=b^{n}a$ is true also when n$\leq$-1. So $ab^{n}=b^{n}a$ for all  n $\in$ $\mathbb{Z}$.


\begin{enumerate}

	\item We have $b^{n}a=ab^{n}$ by (1). We use this as a hypothesis and apply (1)
with a,b,n replaced by $b^{n}, a, m$ respectively. Then we obtain $a^{m}b^{n}=b^{n}a^{m}$
for all m,n $\in$ $\mathbb{Z}$.


If G is not a group but merely a nonempty set with an associative
multiplication on it, the proof remains valid for the case m,n $\in$ $\mathbb{N}$; and
also for the case m = 0 or n = 0, provided there is a unique identity e in
G and we agree to write $a^{0} = e $ for all a $\in$ G:

\end{enumerate}

\end{proof}

\begin{lemma}
Let G be a nonempty set with an associative multiplication
on it. Let a,b $\in$ G.

\begin{enumerate}

	\item 
	If $ab = ba$, then $a^{m}b^{n}=b^{n}a^{m}$ for all m,n $\in$ $\mathbb{N}$. 

	\item 
	If, in addition, there is a unique e $\in$ G such that ce = ec for all c $\in$ G,
and if we put $c^{0}$ = e for all c $\in$ G, then $a^{m}b^{n}=b^{n}a^{m}$ also when m=0 or
n=0.
\end{enumerate}

\end{lemma}

\begin{lemma}
Let G be a nonempty set with an associative multiplication
on it. For any m $\in$ $\mathbb{N}$ and for any  for any $a_{1}, a_{2},\dotsb,a_{m}, b$ $\in$ G such that

\[
	a_{i}b=ba_{i}
	\text{ for all }
	i = 1,2, \dotsb ,m
\]

there holds $(a_{1}a_{2}\dots a_{m})b = b(a_{1}a_{2}\dots a_{m})$.
\end{lemma}

\begin{proof}
By induction on m. The case m = 1 is included in the hypothesis.
Suppose now m $\geq$ 2 and the claim is true for $m-1$. Then

\begin{align*}
	a_{1}a_{2}\dotsb a_{m-1}a_{m})b
	&=((a_{1}a_{2}\dotsb a_{m-1})a_{m})b\\
	&= ((a_{1}a_{2}\dotsb a_{m-1})(a_{m}b)\\
	&= ((a_{1}a_{2}\dotsb a_{m-1})(ba_{m})\\
	&= ((a_{1}a_{2}\dotsb a_{m-1})b)a_{m}\\
	&= (b(a_{1}a_{2}\dotsb a_{m-1}))a_{m}
\end{align*}

\end{proof}

\end{document}