\documentclass[11pt]{amsbook}

\usepackage{../HBSuerDemir}

\begin{document}
% ++++++++++++++++++++++++++++++++++++++
\hPage{b2p2/454}
% ++++++++++++++++++++++++++++++++++++++
where $c$ is an arbitrary constant.
\par The following are SDE:
\begin{align*}
	&(x^{2}+1)\hDif{x} + y\hDif{y} = 0, &(y^{2}+1)dx - e^{x}\hDif{y} = 0 \\
	&r\hDif{\theta} - \theta\hDif{r} = 0, &\frac{\hDif{y}}{\hDif{x}} = \frac{y+1}{x-1} \\
	&y' = (1-x)(y-1), &y' = (2+x-2y-xy) \quad(why?)
\end{align*}
	
\begin{exmp}
	Solve $(y^{2}+1)\hDif{x} = (x^{2}+4)\hDif{y} = 0$
	\begin{hSolution}
		Separating\footnote{It's written as 'Seperating', which is a typo, so I fixed it.} the variables, we have
		\begin{align*}
			\frac{\hDif{x}}{x^{2}+4} - \frac{\hDif{y}}{y^{2}+1} = 0 \\
			\Rightarrow \frac{1}{2} \arctan{\frac{x}{2}} - \arctan{y} = c
		\end{align*}
	\end{hSolution}
\end{exmp}


\subsubsection{Equation Reducible to SDE}
\label{subsubsec:EquationReducibleToSDE}
The $DE$
\begin{align*}
	\frac{\hDif{y}}{\hDif{x}} = f(ax+by+c) \qquad (a, b, c const)
\end{align*}
where f is a function of a single variable is reducible to a $SDE$ upon the substitution
\begin{align*}
	t = ax+by+c
\end{align*}
\par Indeed, differentiation given
\begin{align*}
	{a}^{} \frac{\hDif{t}}{\hDif{x}} &= a+b\frac{\hDif{y}}{\hDif{x}} &\Longrightarrow \frac{\hDif{y}}{\hDif{x}} &= \frac{1}{t}\frac{\hDif{t}}{\hDif{x}} - \frac{a}{t} \\
	\Longrightarrow \: \frac{1}{t}\frac{\hDif{t}}{\hDif{x}} &- \frac{a}{t} = f(t) &\Longrightarrow \frac{\hDif{t}}{\hDif{x}} &- a = f(t)t \\
	\Longrightarrow \quad \frac{\hDif{t}}{\hDif{x}} &= a + f(t)t &\Longrightarrow \hDif{x} &= \frac{\hDif{t}}{a+f(t)\hDif{t}} \quad (SDE)
\end{align*}

\begin{exmp}
	Solve
	\[
		\frac{\hDif{y}}{\hDif{x}} = e^{2x-y+1} + 2x-y+1
	\]
\end{exmp}

\end{document}