\documentclass[11pt]{amsbook}

\usepackage{../HBSuerDemir}

\begin{document}

% ++++++++++++++++++++++++++++++++++++++
\hPage{b2p1/217}
% ++++++++++++++++++++++++++++++++++++++
$\quad(9x^2+18x)-4y^2+(z^2-4z)+13=0$\\
$\Rightarrow 9(x^2+2x)-4y^2+(z-2)^2-4+13=0$\\
$\Rightarrow 9(x+1)^2-9-4y^2+(z-2)^2+9=0$\\
$\Rightarrow 9(x+1)^2-4y^2+(z-2)^2=0$\quad (cone, vertex at (-1, 0, 2))

Since 
	\[
	T=
	\begin{vmatrix}
   	18 & 0 & 0 & 18\\
	0 & -8 & 0 & 0\\
	0 & 0 & 2 & -4\\
	18 & 0 & -4 & 26
	\end{vmatrix}
	=0
	\]
the cone is degenerate.
	\begin{hEnumerateAlpha}
	\item[b)]
	Since there is only one cross term, namely -2xz, the standart equation is obtained by rotating 0xz about 0 by a proper angle $\theta$:
	\[
	(x^2-2xz+z^2)-y^2+2x-4y-2z-3=0 \qquad (1)
	\]
	\[	
tan2\theta = \frac{-2}{1-1} = \infty \quad\Rightarrow\quad \theta = \pi / 4 \quad\Rightarrow\quad cos\theta = sin\theta = \sqrt{2}/2
	\]
	\[
	x=\frac{\sqrt{2}}{2} (x^{\prime}-z^{\prime}),\quad z=\frac{\sqrt{2}}{2} (x^{\prime}+z^{\prime}),\quad y=y^{\prime}.
	\]
	Setting these values in (1), we have
	\[
	\frac{1}{2}(x^{\prime}-z^{\prime})^2-2.\frac{2}{4}({x^{\prime}}^2-{z^{\prime}}^2) + \frac{1}{2} (x^{\prime}+z^{\prime})^2 - {y^{\prime}}^2+\sqrt{2}(x^{\prime}-z^{\prime})-4y^{\prime}-\sqrt{2}(x^{\prime}+z^{\prime})-3=0 
	\]
	\[
	4{z^{\prime}}^2-2{y^{\prime}}^2-8y^{\prime}-4\sqrt{2}z^{\prime}-6=0
	\]
	\[
	2(z^{\prime}-\frac{\sqrt{2}}{2})^2-(y^{\prime}+2)^2=0\quad \text{(two intersecting planes)} 
	\] 
	
	\end{hEnumerateAlpha}




\end{document}  
