\documentclass[11pt]{amsbook}

\usepackage{../HBSuerDemir}

\begin{document}

% ++++++++++++++++++++++++++++++++++++++
\hPage{b2p2/489}
% ++++++++++++++++++++++++++++++++++++++
\begin{exmp}
	Find the GS of
	\[
	y^{\prime\prime\prime}-2y^{\prime\prime}+y^{\prime}=(x+2)+e^x
	\]

\begin{hSolution}
\begin{enumerate}
	\item[1.]
	$\lambda^3-2\lambda^2+2\lambda = 0  \Rightarrow \lambda(\lambda-1)^2=0 \Rightarrow  \lambda_1=0, \lambda_2=1, \lambda_3=1\\
	\Rightarrow y_c = c_1 + c_2 e^x+c_3 x e^x, \qquad \{1, e^x,xe^x\}$
	\item[2.]
	\underline{$f_1(x)=x+1$}. $S_1=\{x+2,\quad1\}$\\
	where 1 is contained in $y_c$. Then
	\[
	{S_1}^\prime = \{x^2+2x,x\}
	\]
	\underline{$f_2(x)=e^x$}: $S_2=\{e^x\}$\\
	$e^x$ is contained in $y_c$. Then
	\[
	{S_2}^\prime = \{x^2 e^x\}
	\]
	So
	\[
	y_p=A(x^2+2x)+Bx+Cx^2 e^x
	\]
	\item[3.] 
		$y_p=Ax^2+(A+B)x+Cx^2e^x$\\
		\begin{tabular}{r|l l}
		1 & ${y_p}^{\prime}$ &$= 2Ax +(A+B)+2Cxe^x+Cx^2e^x$\\
		-2 & $ {y_p}^{\prime\prime}$ &$= 2A + Ce^x + 4Cxe^x + Cx^2e^x$\\
		1 & ${y_p}^{\prime\prime\prime}$ &$= 6C e^x + 6Cxe^x + Cx^2e^x$

		\end{tabular}\\
		\begin{tabular}{lll}
		$(x+2)+e^x $ & = & $2Ax+(A+B) + 2Cxe^x + Cx^2e^x$\\
		&&$-4A - 4C e^x - 8Cxe^x - 2Cx^2e^x$\\
		&&$+6Ce^x+6Cxe^x+Cx^2e^x$\\
		$x+2+e^x$ & = & $2Ax + (B-3A) + 2Ce^x$\\
		\end{tabular}\\
$\Rightarrow$\quad $2A=1$, \quad $B-3A=2$, \quad $2C=1$
\end{enumerate}
\end{hSolution}
\end{exmp}
\end{document}  




























