% Mustafa Alparslan
%X: feyzioglu
%Z: Page 035

\documentclass[11pt]{amsbook}

\usepackage{../HBSuerDemir}	% ------------------------


\begin{document}

% ++++++++++++++++++++++++++++++++++++++
\hPage{feyzioglu/035}
% ++++++++++++++++++++++++++++++++++++++

% =======================================
\section{Divisibility}

In this paragraph, we remind the reader of certain properties of integers concerning divisibility. First we recall the definition.
\begin{cor}
Let  $a,b \in Z$. If $a \neq 0$ and if there is \textnormal{a} $c \in Z$ such that $a*c = b$, then $a$ is called \textnormal{a} divisor or \textnormal{a} factor of $b$, and $b$ is said to be divisible by $a$. We also say $a$ divides $b$.
\end{cor}

We write $a	\mid	 b $ to express that $a$ divides $b$. Whenever we employ the notation $a	\mid	 b$, it will be assumed of course $a\neq 0$. We shall write $a \nmid b$ 	when $a \neq 0$ and $b$ is not divisible by $a$. Thus we have 
$3 \mid 6$, $3 \mid 9$, $2 \mid 8$, $5 \nmid 9$, $5 \mid 10$, 
$3 \nmid 7$, $4 \mid 8$, $-3 \mid 6$, $2 \mid -4$, $-2 \mid -4$.   
The notations $0 \mid b$ and $0 \nmid b$ are meaningles: not true or false, simply undefined.
Some basic properties of divisibility are collected below.

\begin{cor} Lemma: Let \(a,b,c,m,n,m_1,m_2,..., m_s,b_1,b_2,...,b_s \) be integers.

\begin{enumerate}[label={\arabic*.}]

  \item If $a \mid b$, then \( a \mid -b, -a \mid -b, -a \mid b \).
  \item If $a \mid b$ and $b \mid c$, then $a \mid c$.
  \item If $a \mid b$ and $c \neq 0$, then $a*c \mid b*c$.
  \item If  $a*c \mid b*c$, then $a \mid b$.
  \item If $a \mid b$ and $a \mid c$, then $a \mid b + c$.
  \item If $a \mid b$ and $a \mid c$, then $a \mid b - c$.
  \item If $a \mid b$ and $a \mid c$, then $a \mid m*b + n*c$.
  \item If \(a \mid b_1, a \mid b_2,..., a \mid b_s\), then  \(a \mid m_1*b_1 + m_2*b_2 + ... + m_s*b_s\).
  \item If $a \neq 0$, then $a \mid 0$.
  \item $1 \mid a$ and $-1 \mid a$.
  \item If $a \mid b$ and $b \neq 0$, then $|a| \leq |b|$.
  \item If $a \mid b$ and $b \mid a$, then $|a| = |b|$.
\end{enumerate}
\end{cor}

\begin{proof}
\begin{enumerate}[label={\arabic*.}]
\item
If $a \mid b$, then $a \neq 0$ and $a*k = b$ for some $k \in Z$. So $a \neq 0$ and $a*(-k) = -b; \quad a \neq 0$ and $(-a)*k = -b; \quad a \neq 0$ and $(-a)*(-k) = b; \:$ with $k, -k \in Z$. Hence $a \mid -b, -a \mid -b, -a \mid b.$
\end{enumerate}
\end{proof}

% =======================================================
\end{document}  

