\documentclass[11pt]{amsbook}

\usepackage{../HBSuerDemir}

\begin{document}
\hPage{b2p2/308}

\begin{hEnumerateArabic}

    \item [45.] Find the equations of the tangent line to curve of intersection of two surfaces, at given point:
    \begin{hEnumerateAlpha}
        \item $z = x^{2} + y^{2}, \quad z = 2x + 4y + 20, \quad (4, -2, 20)$
        \item $z = \sqrt{25 - 16x^{2}}, \quad z = e^{xy} + 2, \quad (1, 0, 3)$
    \end{hEnumerateAlpha}
    
    \item[46.] Find the point(s) on the surface $z = x^{2} - y^{2}$ at which the tangent plane is parallel to $\vec{V} = (2, 1, 3)$.
    
    \item[47.] Find the points of the surface
    $$x^{\frac{2}{3}} + y^{\frac{2}{3}} + z^{\frac{2}{3}} = 4$$
    at which the normal line is parallel to $\vec{V} = (2, 1, -1)$.
    
    \item[48.] Show that the  tangent plane of the following surfaces at any point passes through a fixed point and find this fixed point:\\
    a) $\frac{(x-1)^{2}}{4} + \frac{(y-2)^{2}}{3} - z^{2} = 0 \qquad$
    b) $\frac{(x-\alpha)^{2}}{a^{2}} + \frac{(y-\beta)^{2}}{b^{2}} + \frac{(c-\gamma)^{2}}{c^{2}} = 0$
    \ifx
        At first, I made the bottom one but then I changed to the upper one to make similar to the original page.
        \begin{hEnumerateAlpha}
            \item $\frac{(x-1)^{2}}{4} + \frac{(y-2)^{2}}{3} - z^{2} = 0$
            \item $\frac{(x-\alpha)^{2}}{a^{2}} + \frac{(y-\beta)^{2}}{b^{2}} + \frac{(c-\gamma)^{2}}{c^{2}} = 0$
        \end{hEnumerateAlpha}
    \fi
    
    \item[49.] Find the equations of the tangent plane and the normal line of the following surfaces at the given point:\\
    a) $z = \ln{xy}, \quad (1, e^{2}, 2) \qquad$
    b) $z = x^{2} + 2xy - y^{2}, \quad (0, 1, -1)$
    \ifx
        At first, I made the bottom one but then I changed to the upper one to make similar to the original page.
        \begin{hEnumerateAlpha}
            \item $z = \ln{xy}, \quad (1, e^{2}, 2)$
            \item $z = x^{2} + 2xy - y^{2}, \quad (0, 1, -1)$
        \end{hEnumerateAlpha}
    \fi
    
    \item[50.] Find the directional derivative of the following function in the given direction at the given point in the positive sense:
    \begin{hEnumerateAlpha}
        \item $z = x^{2} - 2xy \quad $ along $ \quad y = x^{2} \quad $ at $ \quad (2, 4, -12)$
        \item $z = x\ln{\sin{y}} \quad $ along $ \quad y = \frac{\pi}{2}x \quad $ at $ \quad (\frac{1}{3}, \frac{\pi}{6}, \frac{-2}{3})$
    \end{hEnumerateAlpha}
    
    \item[51.] Find the directional derivative of the following function at the given point in the given direction:
    \begin{hEnumerateAlpha}
        \item $w = x\ln{yz} \quad $ at $ \quad A(1, 1, 1) \quad $ toward $ \quad B(, -1, 2)$
        \item $w = e^{x^{2}}\sin{y}\cos{z} \quad $ at $ \quad A(0, \frac{\pi}{2}, 0) \quad $ toward $ \quad B(-1, \frac{\pi}{2}, 2)$
    \end{hEnumerateAlpha}
    
    \item[52.] Same question for:
    \begin{hEnumerateAlpha}
        \item $f (x, y, z) = e^{x}\cos{y} + e^{y}\sin{z} \quad $ at $ \quad P(2, 1, 0) \quad $ toward $ \quad P'(-1, 2, 2)$
        \item $f (x, y, z) = \ln{(x^{2} + z^{2})} + e^{y} \quad $ at $ \quad P(0, 0, 1) \quad $ toward $ \quad P'(-4, 3, 2)$
    \end{hEnumerateAlpha}

\end{hEnumerateArabic}

\end{document}