\documentclass[11pts]{amsbook}
\usepackage{../HBSuerDemir}
\begin{document}
\hPage{466}
\begin{center}
$\frac{dy}{dy}$ = A(x)$y^2$ + B(x)y + C(x) \qquad \qquad \qquad \qquad (1')
\end{center}
so that the derivative is a quadratic expression in y.

\qquad The RDE cannot be sold unless a particular solution is known. If $y_1$ is a PS of (1') the transformation
\begin{center}
y = $y_1$ + u(x)
\end{center}
transforms it to a BDE with a = 2 which in turn, is transformed into a LDE by u=$t^{-1}$. Hence the transformation
\begin{center}
y = $y_1 + \frac{1}{v}$
\end{center}
reduces (1') into a LDE.

\qquad Indeed, 

\qquad \qquad \qquad $\frac{dy_1}{dx} - \frac{v'}{v^2} = {A(y_1+\frac{1}{v})}^2+B(y_1+\frac{1}{v})+C$

\qquad $\Longrightarrow y_1' - \frac{v'}{v^2} = (Ay_1^2 + By_1  + $ C)$ + (\frac{2Ay_1 + B}{v}) + \frac{A}{v^2} +$

\qquad $\Longrightarrow \qquad -v' = (2Ay_1 + B)v + A$

\qquad $\Longrightarrow \qquad v' + (2Ay_1 + B)v = -A(x)$ \qquad \qquad \qquad (LDE)

\begin{exmp}
Given the RDE.

\qquad \qquad y' + $y^2 + 2xy + x^2 + 1 = 0$

a) find a PS of the form $y_1$ = ax (a const)

b) Solve.
\begin{hSolution}
a) a + $a^2x^2 + 2x.ax + x^2 + 1 = 0$

\qquad $\Longrightarrow  (a^2 + 2a + 1)x^2 + (a+1) = 0$

\qquad $\Longrightarrow  a^2 + 2a + 1 = 0, a + 1 = 0 \qquad \Longrightarrow a = -1$

\qquad $\Longrightarrow  y_1 = -x.$
\end{hSolution}
\end{exmp}




\end{document}
