
\documentclass[12pt]{article}
\usepackage{../HBSuerDemir}
\begin{document}
    \hPage{b1p2/293} %page number
    \noindent To prove $T=T'$, multiplying the first row by -h and the second by -k and adding to the last row, we have
        
    \hspace{2.5cm}
    $
    T' = $
    $
    \left |
    \begin{array}{lll}
    2A & B & 2Ah + Bk + D\\
    B  & 2C & Bh + 2Ch + E \\
    D  & E & 2f(h, k)-D h-E'k \\
    \end{array}
    \right |
    $\\
    Now multiplying the first column by -h and the second by -k and adding the last column, we get
        
    \hspace{2.5cm}
    $T' = $
    $ 
    \left |
    \begin{array}{lll}
    2A & B & D\\
    B  & 2C & E \\
    D  & E & 2f(h, k)-D'h-E'k-Dh-Ek \\
    \end{array}
    \right |
    $ \\
    where the element $a_{33}$ is simplified to 2F. Hence $T' = T$. 
    
    Recalling that the coefficients of the transformed equation under a rotation are
    \begin{center}
        \begin{tabular}{ l l}
            $A' = Ac^2 + Bcs + Cs^2$,& $D' = Dc + Es$, \\
            $B' = B(c^2-s^2)-2(A-C)cs$, & $E' = -Ds + Ec$, \\
            $C' = As^2 - Bcs + Cc^2$, & $F' = F$, \\
        \end{tabular}
    \end{center}
    where c, s stand for $\cos\theta$, $\sin\theta$, we have
    \begin{center}
        $H' = A' + C' = A(c^2+s^2) + C(s^2+c^2) = A + C = H$
    \end{center}
    
    To prove the invariance of $\Delta$, we write A', B', C' in terms of $\cos2\theta$,  $\sin2\theta$ by the use of $2\cos^2\theta=1+\cos2\theta$, $2\sin^2\theta=1-\cos2\theta$:
    \begin{align*}
        2A' &= B\sin2\theta + (A-C)\cos2\theta + A + C\\
        B' &= B\cos2\theta + (A-C)\sin2\theta\\
        2C' &= B\sin2\theta + (A-C)\cos2\theta + A + C,
    \end{align*}
    we have 
    \begin{align*}
        \Delta'&=B'^2-4A'C'\\
        &=[B\cos2\theta-(A-C)\sin2\theta]^2-[(A+C)^2-(B\sin2\theta+(A-C)\cos2\theta)^2]\\
        &=B^2 + (A-C)^2-(A+C)^2 = B^2-4AC^2 = \Delta
    \end{align*}
    
    The invariance of T is proved as follows:
\end{document}