\documentclass[11pt]{amsbook}

\usepackage{../HBSuerDemir}	% ------------------------

\begin{document}

% ++++++++++++++++++++++++++++++++++++++
\hPage{b1p2/356}
% ++++++++++++++++++++++++++++++++++++++


% =======================================
\begin{proof}
	Let $F(x) = \int_{a}^{x} \! f(t) \, \hDif t$. Then
	
	\begin{align*}
		F(x+h) - F(x) &= \int_{a}^{x+h} \! f(t) \, \hDif{t} - \int_{a}^{x} \! f(t) \, \hDif{t} \\
		&= \int_{a}^{x+h} \! f(t) \, \hDif{t} + \int_{x}^{a} \! f(t) \, \hDif{t}\\
		&= \int_{x}^{x+h} \! f(t) \, \hDif{t} \\
		&= \Big((x+h)-x\Big) f(c), \quad\quad x < c < x+h
	\end{align*}
	
	\noindent by the MVT for integral. Hence
	
	\begin{align*}
		\frac{F(x+h) - F(x)}{h} &= f(c) = f(x+ \theta h), \quad\quad 0< \theta < 1 \\
		\lim_{h \to 0} \frac{F(x+h) - F(x)}{h} &= \lim_{h \to 0} f(x + \theta h) = f(x).
	\end{align*}
\end{proof}

\begin{thm}[F.T. of integral calculus]
	If $f(x) \epsilon C(a,b)$ and $F(x)$ is a primitive of $f(x)$, then

	\begin{equation*}
		\int_{a}^{b} \! f(x) \, \hDif{x} = F(b) - F(a)
	\end{equation*}
\end{thm}

\begin{proof}
	Since $D \int_{a}^{x} \! f(t) \, \hDif{t} = f(x)$ by previous theorem and $DF(x)~=~f(x)$,  % "~" placed to keep equation from getting splitted in half
	then $\int_{a}^{x} \! f(t) \, \hDif{t}$ differs from $F(x)$ by a constant:

	\begin{equation*}
		\int_{a}^{x} \! f(t) \, \hDif{t} = F(x) + c
	\end{equation*}

	\noindent Now

	\begin{align*}
		x &= a \quad\Longrightarrow\quad 0 = F(a) + c \quad\Longrightarrow\quad c = -F(a),\\
		x &= b \quad\Longrightarrow\quad \int_{a}^{b} \! f(t) \, \hDif{t} = F(b) + c = F(b) - F(a).
	\end{align*}
\end{proof}

\begin{notation}
		 $\int_{a}^{b} \! f(t) \, \hDif{t} = F(b) - F(a) = F(x)$
		$\begin{vmatrix}
			x = b\\
			& = F(x)\\
			x = a 
		\end{vmatrix}_{a}^{b}$
\end{notation}

In view of this theorem, evaluation of a definite integral reduces to that of an indefinite integral. 
It is to be noted that if the evaluation is done by substitution, the new limits

% =======================================================
\end{document}  
