

\documentclass[11pt]{amsbook}

\usepackage{../HBSuerDemir}	% ------------------------


\begin{document}

% ++++++++++++++++++++++++++++++++++++++
\hPage{feyzioglu-085}
% ++++++++++++++++++++++++++++++++++++++
\begin{proof} Writing ($e'$) with $a^{-1}$ in place of $a$ and using (2), we get $(a^{m})^{-n}$=$[(a^{m})^{-1}]^{n}$=
$(a^{-m})^{n}$=$[(a^{-1})^{m}]^{n}$=$(a^{-1})^{mn}$=$a^{-(mn)}$=$a^{m(-n)}$. This proves $(i)$. We also get $(a^{-m})^{n}$=$a^{-(mn)}$=$a^{-(m)n}$. This proves $(ii)$. Finally, we have $(a^{-m})^{-n}$=$[(a^{m})^{-1}]^{-n}$=
$([(a^{m})^{-1}]^{-1})^{n}$=$(a^{m})^{n}$=$a^{mn}$=$a^{(-m)(-n)}$. This proves $(iii)$.

Thus $(a^{m})^{n}$=$a^{mn}$ for all $m,n \in \hSoZ$. 
\bigbreak
The proof is complete.
\end{proof}

\begin{lem} $Let$ $G$ $be$ $a$ $group$ $and$ $a_{1},a_{2},\dotsc,a_{n}$ $\in$ $G$. Then
\begin{center}
 $(a_{1} a_{2} \dotsc a_{n})^{-1}$=$a_{n}^{-1} \dotsc a_{2}^{-1} a_{1}^{-1}$
\end{center}

\begin{proof} By induction on $n$. If $n$ = 2, the assertion is true by Lemma 8.2(2). Suppose now $n \in \hSoN$, $n \geq 3$ and $(a_{1} a_{2} \dotsc a_{n-1})^{-1}$=$a_{n-1}^{-1} \dotsc a_{2}^{-1} a_{1}^{-1}$. Then
\begin{align*}
 (a_{1} a_{2} \dotsc a_{n-1} a_{n})^{-1} & = ((a_{1} a_{2} \dotsc a_{n-1}) a_{n})^{-1} \\
& = a_{n}^{-1}(a_{1} a_{2} \dotsc a_{n-1})^{-1} \\
& = a_{n}^{-1}(a_{n-1}^{-1} \dotsc  a_{2}^{-1} a_{1}^{-1}) \\
& = a_{n}^{-1} a_{n-1}^{-1} \dotsc  a_{2}^{-1} a_{1}^{-1} 
\end{align*}

as was to be proved.
\end{proof}

Lemma 8.8 gives an alternative proof of $(a^{-1})^{m}$=$(a^{m})^{-1}$. When our group is commutative, we have additional results for example $a^{m}b^{n}$=$b^{n}a^{m}$.
\end{lem}

\begin{lem} $Let$ $G$ $be$ $a$ $group$ $and$ $a,b \in G$. $If$ $ab=ba$ $then$
\begin{flalign*}
&(1) ab^{n} = b^{n}a; & \\
&(2) a^{m}b^{n} = b^{n}a^{m}; 
\end{flalign*}
for all $m,n \in \hSoZ $.

\begin{proof} (1) We prove $ab^{n}$=$b^{n}a$: The case n=0 is trivial. Also $ab^{1}=ab=ba=b^{1}a$ by hypothesis and the claim is true for $n = 1$. Suppose now $n \in \hSoN$, $n \geq 2$ and the claim is proved for $n-1$, so that $ab^{n-1}$=$b^{n-1}a$. Then $ab^{n}=a(b^{n-1}b)=(ab^{n-1})b=(b^{n-1}a)b=b^{n-1}(ab)=b^{n-1}(ba)=(b^{n-1}b)a=b^{n}a$. By induction, $ab^{n}=b^{n}a$ for all $n \in \hSoN$.
\end{proof}
\end{lem}
\end{document}  



