\documentclass[11pt]{amsbook}
 
 

\usepackage{../HBSuerDemir}

\begin{document}

\hPage{feyziohlu-079}

\begin{proof}
	\noindent
	(1) If $ab = ac$, we multiply by $a^{-1}$  on the left and get 			$a^{-1}(ab)=a^{-1}(ac)$. Using associativity, -we obtain $(a^{-1}		a)b=(a^{-1}a)c$. So $1b = lc$. Since $1$ is  the identity element 		of $G$, we finally get $b = c$.\\
 	\par\noindent
 	(2) The proof of (2) is similar and is left to the reader. 
\end{proof}
 

\par\noindent \\\\
	We must be careful when we want to use Lemma 8.1 to make cancel- 		lation. If the group is not commutative, left multiplication by an 	element  and right multiplication by the same element give in 			general different results.In the proof of Lemma 8.l, we multiplied 	by $a^{-1}$ on the same side. We cannot conclude $b = c$ from $ab 		= ca$, for instance. Indeed, we have 
\par
	$ab = ca$  $\Longrightarrow$  $a^{-1}(ab)=a^{-1}(ac)$   $				\Longrightarrow$  $(a^{-1}a)b=(a^{-1}c)a$  $\Longrightarrow$ $b = 		a^{-1}ca$
\par\noindent
	and this is all we can say.In general $a^{-1}ca \neq c$ so $b\neq 		c$.You must always Â·make sure that you cancel on the same side.\\
\par\noindent
	Cancellations are multiplications by inverse elements. We now 			evaluate the inverse of an inverse, and the inverse of a product.\\\\
\begin{lem} 
 	Let G be a group and let $a,b\in G$. Then 
 	\par\noindent
  		(1) ${(a^{-1})^{-1}}=a$,
 	\par\noindent
 		(2) $(ab)^{-1} = b^{-1}a^{-1}$.
\end{lem}

\begin{proof}
	\noindent
		(1) $aa^{-1}=l$ by the definition of $a^{-1}$.So a is a left 			inverse of $a^{-1}$.So a is the inverse of $a^{-1}$(Lemma 				7.3).\\ 
	\par\noindent
 		(2) (ab)($b^{-l} a^{-1}$) = a(b( $b^{-l}$ $a^{-1}$ )) = a((b  			$b^{-1}$ ) $a^{-1}$) = a(1$a^{-1}$) = a $a^{-1}$ =1, and so 			$b^{-l}$ $a^{-1}$  is the inverse of a b. 
\end{proof}

\par\noindent\\\\
	Therefore, the inverse of the inverse of an element is the element 	itself. Also, the inverse of a product is the product of the 			inverses, but in the reverse order. Do not write ${(ab)}^{-1}			=a^{-1}b^{-1}$. This is wrong unless $a^{-1}b^{-1}=b^{-1}a^{-1}$, 		which is equivalent to $ab=ba$ (why?) and which is not true in 			general. 
 
    
\end{document}