\documentclass[11pt]{amsbook}
\usepackage{../HBSuerDemir}

\begin{document}
	\hPage{b2p1/203}
	\begin{hSolution}
		\indent a) Since $\ell$ passes through $P_0$ and its direction numbers are $x_0 - f(t)$, $y_0 - g(t)$, $z_o - h(f)$, one has
		\begin{equation*}
		    S: \frac{x-x_0}{x_0 - f(t)} = \frac{y - y_0}{y_0 - g(t)} = \frac{z - z_0}{z_0 - h(t)}
		\end{equation*}
		as the \underline{symmetric equations} of the cone.\\
		\indent When t is eliminated one obtains 
		\begin{equation*}
		    S : H(x, y, z) = 0		  
		\end{equation*}
		\indent b) If P(x, y, z) is any point on the generatrix $\ell$ (a point of S), then any other point $Q$ on $\ell$ has coordinates 
		$$ \frac{x + tx_0}{1 + t} , \frac{y + ty_0}{1 + t} , \frac{z + tz_0}{1 + t}$$
		Setting these on $F$ = 0, $G$ = 0 and elinimating $t$ one gets 
		\begin{equation*}
		    S: H(x, y, z) = 0
		\end{equation*}
	\end{hSolution}
	\begin{exmp}
	    Obtain the cartesian equations of the cones defined by 
	    \begin{align*}
	        &a) P_0(0, 0, 1),   &&r: x = 2t, \ \  y=t^2 , z=0\\
	        &b) P_0(0, 0, 1),   &&r: x^2 = 2z,\ \  y-z = 1
	    \end{align*}
	\end{exmp}
	
	\begin{hSolution}
	    $\begin{aligned}[t]
	         &a)   \frac{x}{2t} = \frac{y}{t^2} = \frac{z-1}{-1}\\
            &\Rightarrow t^2x = 2ty,   -x = 2t(z-1) \\ &\Rightarrow tx = 2y, \ \  -x = 2t(z-1)\\
            &\Rightarrow -x = \frac{4y}{x} (z-1) \Rightarrow -x^2 = 4y(z-1)\\
            &\Rightarrow x^2 + 4yz -4y = 0
        \end{aligned}$

	\end{hSolution}
\end{document}