\documentclass[11pt]{amsbook}
\usepackage{../HBSuerDemir}

\begin{document}
	\hPage{b2p2/471}
	
	\begin{enumerate}
        \item[19.] Same question for:\\
        a) $dy = (\frac{y}{x} - \csc ^2 \frac{y}{x})dx$,   b)$(3x^2 + 2xy + 4y^2)dx + (20x^2 + 6xy + y^2) dy = 0$ 
        \item[20.] Find the PS under the given condition:\\
        a) $(x+y) dy - ydx = 0;\ \  y(0) = 1$\\
        b) $(x^2 + 2xy - y^2) dx + (y^2 + 2xy - 2x^2)dy = 0,\ \ \ y(0) = 3$
        \item[21.] Find the GS of the following EDE:\\
        a)$(2x^2 + 5xy^2)dx + (5x^2y - 2y^4)dy = 0$\\
        b)$\sec^2x \tan y dx  + \sec^2y \ tanx\  dy = 0$
        \item[22.] a) $\arcsin y dx + \frac{x + 2\sqrt{1-y^2} \cos y}{\sqrt{1-y^2}} dy = 0$\\
        b)$(x \ln y + y \ln x + y)dx + ( \frac{x^2}{2y} + x \ln x)dy = 0$
        \item[23.] Same question for:\\
        a) $(y \cosh xy + \cosh y)dx + (x \cosh xy + x \sinh y)dy = 0$\\
        b) $(\sin x + \sin y)dx + (x \cos y + \cos y)dy = 0$
        \item[24.] Find the PS passing through the given point:\\
        a) $(2x \sin y + 2x + 3y \cos x)dx + (x^2 \cos y + 3 \sin x)dy = 0, \ \ \ \ (\pi /2, 0)$\\
        b) $(y e ^{2x} - 3x e^{2y}) dx + (\frac{1}{2} e ^{2x} - 3x^2 e^{2y} - e^y)dy = 0; \ \ \ \ \  (1,0)$ 
        \item[25.] Find an integrating factor $\mu (xy)$ and solve
        $$ x dy + y dx = x^2 + y^2 dx $$
        \item[26.]  Find the GS of the following DE by finding and integrating factor:\\
        a) $ dx + ( x  \tan y -2 \sec y) dy = 0$ \ \ \ b)$(2-xy)y dx + (2 + xy) xdy =0$
        \item[27.] Find the GS:
    \end{enumerate}
\end{document}
